theories/Coherence/AllocationAlgoCorrect.v
@@ -27,9 +27,9 @@ Proof.
   intros; unfold least_fresh_P; cases; try omega; eauto.
 Qed.
 
-Definition sep (c:var) (G:set var) (ϱ:Map [var,var]) :=
-  (forall x, x ∈ G -> ~ x <= c -> findt ϱ 0 x === x)
-  /\ (forall x, x ∈ G -> x <= c -> findt ϱ 0 x <= c).
+Definition sep (c:var) (G:set var) (ϱ:var -> var) :=
+  (forall x, x ∈ G -> ~ x <= c -> ϱ x === x)
+  /\ (forall x, x ∈ G -> x <= c -> ϱ x <= c).
 
 Instance sep_morphism_impl
   : Proper (eq ==> Equal ==> eq ==> impl) sep.
@@ -70,7 +70,7 @@ Proof.
 Qed.
 
 Lemma sep_agree c D ϱ ϱ'
-  : agree_on eq D (findt ϱ 0) (findt ϱ' 0)
+  : agree_on eq D ϱ ϱ'
     -> sep c D ϱ
     -> sep c D ϱ'.
 Proof.
@@ -79,11 +79,12 @@ Proof.
   - rewrite <- AGR; eauto.
 Qed.
 
+
 Hint Resolve sep_incl sep_agree.
 
-Lemma sep_lookup_set c (G:set var) (ϱ:Map [var,var]) x
+Lemma sep_lookup_set c (G:set var) (ϱ:var -> var) x
       (SEP:sep c G ϱ) (NotIn:x ∉ G)
-  : ~ x <= c -> x ∉ lookup_set (findt ϱ 0) G.
+  : ~ x <= c -> x ∉ lookup_set ϱ G.
 Proof.
   destruct SEP as [GT LE].
   intros Gt. unfold lookup_set; intro In.
@@ -94,10 +95,14 @@ Proof.
   - exploit GT; eauto.
 Qed.
 
-Lemma sep_update c lv x ϱ
-      (SEP : sep c (lv \ singleton x) ϱ)
-      (CARD : cardinal (map (findt ϱ 0) (lv \ singleton x)) <= c)
-  : sep c lv (ϱ [-x <- least_fresh_P c (map (findt ϱ 0) (lv \ singleton x)) x -]).
+Print Scopes.
+
+Require Import MapNotations.
+
+Lemma sep_update c lv (x:var) (ϱ:Map[var,var])
+      (SEP : sep c (lv \ singleton x) (findt ϱ 0))
+      (CARD : cardinal (filter (fun x => B[x <= c]) (map (findt ϱ 0) (lv \ singleton x))) < c)
+  : sep c lv (findt (ϱ [-x <- least_fresh_P c (map (findt ϱ 0) (lv \ singleton x)) x -]) 0).
 Proof.
   destruct SEP as [GT LE].
   split; intros.
@@ -112,8 +117,8 @@ Proof.
     decide (x === x0).
     + rewrite MapFacts.add_eq_o; eauto.
       rewrite least_fresh_P_le.
-      * rewrite least_fresh_small.
-        eapply CARD.
+      * rewrite (@least_fresh_filter_small c); eauto.
+        unfold findt in CARD. unfold var in *. omega.
       * hnf in e; congruence.
     + rewrite MapFacts.add_neq_o; eauto.
       cases; try omega.
@@ -123,7 +128,7 @@ Proof.
 Qed.
 
 Lemma sep_nd c G ϱ G'
-      (SEP:sep c G ϱ) (Disj: disj G' G)
+      (SEP:sep c G (findt ϱ 0)) (Disj: disj G' G)
   : forall x : nat, x > c -> x ∈ G' -> x ∈ map (findt ϱ 0) G -> False.
 Proof.
   intros. cset_tac. destruct SEP as [GT LE].
@@ -133,20 +138,187 @@ Proof.
     eapply Disj; eauto; congruence.
 Qed.
 
+Lemma sep_lookup_list c (G s:set var) (ϱ:var -> var) x
+      (SEP:sep c (G \ s) ϱ)
+  : x > c -> x ∈ s -> x ∉ map ϱ (G \ s).
+Proof.
+  destruct SEP as [GT LE].
+  intros Gt. intros In InMap.
+  eapply map_iff in InMap; eauto.
+  destruct InMap as [y [In' EQ]]. hnf in EQ; subst.
+  decide (y <= c).
+  - exploit LE; eauto. omega.
+  - cset_tac.
+Qed.
+
+Lemma sep_update_list c ϱ lv Z
+      (AL:forall x, x > c -> x ∈ of_list Z -> x ∈ map (findt ϱ 0) (lv \ of_list Z) -> False)
+      (ND: NoDupA eq Z)
+      (Card: crd c (map (findt ϱ 0) (lv \ of_list Z)) Z)
+      (SEP:sep c (lv \ of_list Z) (findt ϱ 0))
+  : sep c lv (findt (ϱ [-Z <-- fresh_list_P c (map (findt ϱ 0) (lv \ of_list Z)) Z -]) 0).
+Proof.
+  destruct SEP as [GT LE].
+  eapply sep_agree.
+  setoid_rewrite <- map_update_list_update_agree'; eauto with len.
+  reflexivity.
+  split; intros.
+  - decide (x ∈ of_list Z).
+    + edestruct update_with_list_lookup_in_list; try eapply i; dcr.
+      Focus 2.
+      rewrite H4. cset_tac.
+      edestruct fresh_list_get; try eapply H3; inv_get; eauto.
+      dcr. inv_get. exfalso; eauto.
+      eauto with len.
+    + rewrite lookup_set_update_not_in_Z; eauto.
+      eapply GT; eauto with cset. cset_tac.
+  - decide (x ∈ of_list Z).
+    + edestruct update_with_list_lookup_in_list; try eapply i; dcr.
+      Focus 2.
+      rewrite H4. cset_tac.
+      edestruct fresh_list_get; try eapply H3; inv_get; eauto.
+      dcr. inv_get.
+      eauto with len.
+    + rewrite lookup_set_update_not_in_Z; eauto.
+      eapply LE; eauto with cset. cset_tac.
+Qed.
+
 (** ** the algorithm produces a locally injective renaming *)
 
-Lemma regAssign_correct c (ϱ:Map [var,var]) ZL Lv s alv ϱ' al
+Require Import AnnP.
+Definition bounded_below
+           (c : nat)
+           (k : nat)
+  : ⦃nat⦄ -> Prop
+  :=
+    fun a => cardinal (filter (fun x => B[x <= c]) a) <= k.
+
+
+Instance bounded_in_equal_morph
+  : Proper (eq ==> eq ==> Equal ==> iff) bounded_below.
+Proof.
+  unfold Proper, respectful, bounded_below; intros; subst.
+  rewrite H1. reflexivity.
+Qed.
+
+Instance bounded_in_subset_morph
+  : Proper (eq ==> eq ==> Equal ==> impl) bounded_below.
+Proof.
+  unfold Proper, respectful, bounded_below, impl, flip; intros; subst.
+  rewrite <- H1. rewrite <- H2. reflexivity.
+Qed.
+
+
+Instance bounded_in_equal_ptw
+  : Proper (eq ==> eq ==> pointwise_relation _ iff) bounded_below.
+Proof.
+  unfold Proper, respectful, pointwise_relation; intros; subst.
+  reflexivity.
+Qed.
+
+Instance bounded_in_impl_ptw'
+  : Proper (eq ==> eq ==> pointwise_relation _ impl) bounded_below.
+Proof.
+  unfold Proper, respectful, pointwise_relation, impl, flip; intros; subst.
+  eauto.
+Qed.
+
+Instance ann_P_impl A
+  : Proper (@pointwise_relation _ _ impl ==> eq ==> impl) (@ann_P A).
+Proof.
+  unfold Proper, respectful, impl; intros; subst.
+  general induction H1; eauto using ann_P.
+Qed.
+
+Instance ann_P_iff A
+  : Proper (@pointwise_relation _ _ iff ==> eq ==> iff) (@ann_P A).
+Proof.
+  unfold Proper, respectful, impl; intros; subst; split; intros.
+  eapply ann_P_impl; eauto.
+  eapply pointwise_subrelation; eauto using iff_impl_subrelation.
+  eapply ann_P_impl; eauto.
+  eapply pointwise_subrelation; eauto using iff_impl_subrelation.
+  eapply pointwise_symmetric; eauto using CRelationClasses.iff_Symmetric.
+Qed.
+
+Lemma filter_difference X `{OrderedType X} (p:X->bool) `{Proper _ (_eq ==> eq) p} s t
+  : filter p (s \ t) [=] filter p s \ filter p t.
+Proof.
+  cset_tac. eapply H3; cset_tac.
+Qed.
+
+Lemma sep_filter_map_comm (c:var) lv (ϱ:var -> var)
+  : sep c lv ϱ
+    -> map ϱ (filter (fun x => B[x <= c]) lv) [=] filter (fun x => B[x <= c]) (map ϱ lv).
+Proof.
+  intros [GT LE]. cset_tac.
+  - eexists x; cset_tac.
+    exploit GT; eauto. cset_tac. omega.
+Qed.
+
+Lemma subset_filter X `{OrderedType X} (p:X->bool) `{Proper _ (_eq ==> eq) p} (lv lv':set X)
+  : lv ⊆ lv'
+    -> filter p lv ⊆ filter p lv'.
+Proof.
+  cset_tac.
+Qed.
+
+Lemma filter_get X (p:X->bool) (Z:list X) x n
+  : get Z n x
+    -> p x
+    -> { n : nat | get (List.filter p Z) n x }.
+Proof.
+  intros. eapply get_getT in H.
+  general induction H; simpl; cases; eauto using get.
+  edestruct IHgetT; eauto using get.
+Qed.
+
+Lemma of_list_filter X `{OrderedType X} (p:X->bool) `{Proper _ (_eq ==> eq) p} L
+  : of_list (List.filter p L) [=] filter p (of_list L).
+Proof.
+  cset_tac.
+  - eapply of_list_get_first in H1; dcr; cset_tac; inv_get.
+    rewrite H3. eapply get_in_of_list; eauto.
+  - eapply of_list_get_first in H1; dcr; cset_tac; inv_get.
+    rewrite H3. cset_tac.
+  - eapply of_list_get_first in H2; dcr; cset_tac; inv_get.
+    rewrite H4 in *.
+    edestruct filter_get; eauto.
+    eapply get_in_of_list; eauto.
+Qed.
+
+
+Lemma crd_of_list (c:var) k (LT:k < c) (lv:set var) Z ϱ
+      (SEP:sep c (lv \ of_list Z) ϱ)
+      (Card:cardinal (filter (fun x => B[x <= c]) lv) <= k)
+      (Incl: of_list Z ⊆ lv)
+  : crd c (map ϱ (lv \ of_list Z)) Z.
+Proof.
+  unfold crd. rewrite <- sep_filter_map_comm; eauto.
+  rewrite cardinal_map; eauto.
+  rewrite filter_difference; [|clear; intuition].
+  rewrite cardinal_difference'.
+  - unfold var in *.
+    assert (cardinal (filter (fun x => B[x <= c]) lv) >=
+            cardinal (filter (fun x => B[x <= c]) (of_list Z))). {
+      eapply subset_cardinal. eapply subset_filter. clear; intuition. eauto.
+    }
+    unfold var in *. rewrite of_list_filter. omega. clear; intuition.
+  - eapply subset_filter; eauto.
+Qed.
+Lemma regAssign_correct k c (LE:k < c) (ϱ:Map [var,var]) ZL Lv s alv ϱ' al
       (LS:live_sound FunctionalAndImperative ZL Lv s alv)
       (inj:injective_on (getAnn alv) (findt ϱ 0))
-      (SEP:sep c (getAnn alv) ϱ)
+      (SEP:sep c (getAnn alv) (findt ϱ 0))
       (allocOK:regAssign c s alv ϱ = Success ϱ')
       (incl:getAnn alv ⊆ fst (getAnn al))
       (sd:renamedApart s al)
+      (BND:ann_P (bounded_below c k) alv)
 : locally_inj (findt ϱ' 0) s alv.
 Proof.
   intros.
-  general induction LS; simpl in *; try monadS_inv allocOK; invt renamedApart;
-  pe_rewrite; eauto 10 using locally_inj, injective_on_incl.
+  general induction LS; simpl in *; try monadS_inv allocOK; invt renamedApart; invt ann_P;
+    pe_rewrite; simpl in *.
   - exploit IHLS; try eapply allocOK; pe_rewrite; eauto with cset.
     + eapply injective_on_agree; [| eapply map_update_update_agree].
       eapply injective_on_incl.
@@ -155,7 +327,9 @@ Proof.
       eapply sep_lookup_set; eauto.
       eauto with cset.
     + eapply sep_update; eauto.
-      admit.
+      hnf in H4. rewrite <- sep_filter_map_comm; eauto.
+      rewrite cardinal_map; eauto.
+      rewrite H0. unfold var in *. omega.
     + pe_rewrite. eauto with cset.
     + exploit regAssign_renamedApart_agree;
       try eapply allocOK; simpl; eauto using live_sound.
@@ -173,7 +347,7 @@ Proof.
       try eapply EQ0; simpl; eauto using live_sound.
     pe_rewrite.
     simpl in *.
-    exploit IHLS1; eauto using injective_on_incl.
+    exploit IHLS1; try eapply EQ; eauto using injective_on_incl.
     rewrite H11; simpl. rewrite <- incl; eauto.
     exploit IHLS2; try eapply EQ0; eauto using injective_on_incl.
     eapply injective_on_incl; eauto.
@@ -187,11 +361,13 @@ Proof.
     rewrite H11; simpl; eauto.
     exploit regAssign_renamedApart_agree'; try eapply EQ0; simpl; eauto using live_sound.
     pe_rewrite.
-    eapply agree_on_incl. eapply H13. instantiate (1:=D ∪ Ds).
+    eapply agree_on_incl. eauto. instantiate (1:=D ∪ Ds).
     pose proof (renamedApart_disj H9).
     pe_rewrite.
-    revert H6 H14; clear_all; cset_tac; intuition; eauto.
-    rewrite H11; simpl. rewrite <- incl; eauto.
+    revert H6 H17; clear_all; cset_tac; intuition; eauto.
+    pe_rewrite. rewrite <- incl; eauto.
+  - econstructor; eauto.
+  - econstructor; eauto.
 
   - exploit regAssign_renamedApart_agreeF;
     eauto using regAssign_renamedApart_agree'. reflexivity.
@@ -205,10 +381,10 @@ Proof.
       intros; inv_get. edestruct H8; eauto; dcr.
       unfold defVars. symmetry. eapply disj_app; split; eauto.
       symmetry; eauto.
-      exploit H7; eauto. eapply renamedApart_disj in H17.
-      eapply disj_1_incl; eauto. rewrite H16. eauto with cset.
+      exploit H7; eauto. eapply renamedApart_disj in H20.
+      eapply disj_1_incl; eauto. rewrite H19. eauto with cset.
     }
-    exploit IHLS; try eapply EQ0; eauto.
+    exploit (IHLS k c); try eapply EQ0; eauto.
     + eapply injective_on_incl; eauto.
       eapply injective_on_agree; eauto.
     + pe_rewrite. etransitivity; eauto.
@@ -222,11 +398,11 @@ Proof.
       * {
           intros. edestruct get_length_eq; try eapply H6; eauto.
           edestruct (regAssignF_get c (fst (getAnn x0) ∪ snd (getAnn x0) ∪ getAnn alv)); eauto; dcr.
-          rewrite <- map_update_list_update_agree in H21; eauto.
-          exploit H1; try eapply H19; eauto.
+          rewrite <- map_update_list_update_agree in H24; eauto.
+          exploit (H1 _ _ _ H17 H18 k c); try eapply H19; eauto.
           - assert (getAnn alv \ of_list (fst Zs) ∪ of_list (fst Zs) [=] getAnn alv).
             edestruct H2; eauto.
-            revert H17; clear_all; cset_tac; intuition.
+            revert H20; clear_all; cset_tac; intuition.
             eapply injective_on_agree.
             Focus 2.
             eapply agree_on_incl.
@@ -234,7 +410,7 @@ Proof.
             rewrite disj_minus_eq; eauto.
             eapply renamedApart_disj in sd.
             simpl in *.
-            rewrite <- H17. symmetry. rewrite disj_app. split; symmetry.
+            rewrite <- H20. symmetry. rewrite disj_app. split; symmetry.
             eapply disj_1_incl. eapply disj_2_incl. eapply sd.
             rewrite <- H13. eapply incl_union_left.
             hnf; intros ? A. eapply list_union_get in A. destruct A. dcr.
@@ -245,7 +421,7 @@ Proof.
             eapply disj_1_incl.
             eapply defVars_take_disj; eauto. unfold defVars.
             eauto with cset.
-            setoid_rewrite <- H17 at 1.
+            setoid_rewrite <- H20 at 1.
             eapply injective_on_fresh_list; eauto with len.
             eapply injective_on_incl; eauto.
             eapply H2; eauto.
@@ -254,28 +430,52 @@ Proof.
             eapply sep_nd; eauto.
             edestruct H2; eauto. clear; hnf; intros; cset_tac.
             edestruct H8; eauto.
-            admit.
+            edestruct H2; eauto; dcr.
+            exploit H15; eauto. eapply ann_P_get in H26. hnf in H26.
+            eapply crd_of_list; eauto.
             reflexivity.
             edestruct H8; eauto.
             eapply fresh_list_nodup; eauto.
             eapply sep_nd; eauto.
             edestruct H2; eauto. clear; hnf; intros; cset_tac.
             edestruct H8; eauto.
-            admit.
+            edestruct H2; eauto; dcr.
+            eapply crd_of_list; eauto.
+            exploit H15; eauto. eapply ann_P_get in H26. eauto.
           - edestruct H2; eauto.
-            rewrite map_update_list_update_agree' in H21; eauto with len.
-            admit.
-          - edestruct H8; eauto; dcr. rewrite H17.
-            exploit H2; eauto; dcr. rewrite incl in H26; simpl in *.
-            rewrite <- H26. clear_all; cset_tac; intuition.
-          - eapply locally_inj_live_agree; try eapply H17; eauto.
-            eapply regAssign_renamedApart_agreeF in H18;
+            rewrite map_update_list_update_agree' in H24; eauto with len.
+            eapply sep_agree.
+            eapply agree_on_incl; eauto.
+            edestruct H8; eauto; dcr. rewrite H25. rewrite <- incl. rewrite <- H23.
+            eapply not_incl_minus. clear; cset_tac.
+            assert (getAnn alv [=] of_list (fst Zs) ∪ getAnn alv \ of_list (fst Zs)). {
+              revert H20; clear; cset_tac.
+            }
+            rewrite H26. symmetry; eapply disj_app; split.
+            symmetry. eapply disj_1_incl.
+            eapply defVars_take_disj; eauto. unfold defVars. cset_tac.
+            symmetry.
+
+            eapply disj_1_incl. eapply D_take_disj; eauto.
+            rewrite <- incl, <- H23. eauto.
+            edestruct H8; eauto; dcr.
+            eapply sep_update_list; eauto.
+            intros ? ? ?.
+            eapply sep_lookup_list; eauto using sep_incl.
+            edestruct H2; eauto; dcr.
+            eapply crd_of_list; eauto.
+            exploit H15; eauto. eapply ann_P_get in H31. eauto.
+          - edestruct H8; eauto; dcr. rewrite H20.
+            exploit H2; eauto; dcr. rewrite incl in H29; simpl in *.
+            rewrite <- H29. clear_all; cset_tac; intuition.
+          - eapply locally_inj_live_agree; try eapply H20; eauto.
+            eapply regAssign_renamedApart_agreeF in H21;
               eauto using get_drop, drop_length_stable; try reflexivity.
             + eapply regAssign_renamedApart_agree' in EQ0; simpl; eauto using live_sound.
               etransitivity; eapply agree_on_incl; try eassumption.
               * rewrite disj_minus_eq. reflexivity.
                 {
-                  edestruct H8; eauto; dcr. rewrite H20.
+                  edestruct H8; eauto; dcr. rewrite H23.
                   rewrite union_comm. rewrite <- union_assoc.
                   symmetry; rewrite disj_app; split; symmetry.
                   - eapply disj_1_incl. eapply defVars_drop_disj; eauto.
@@ -289,7 +489,7 @@ Proof.
               * pe_rewrite.
                 rewrite disj_minus_eq. reflexivity.
                 {
-                  edestruct H8; eauto; dcr. rewrite H20.
+                  edestruct H8; eauto; dcr. rewrite H23.
                   rewrite union_comm. rewrite <- union_assoc.
                   symmetry; rewrite disj_app; split; symmetry.
                   rewrite union_comm; eauto.
@@ -297,9 +497,9 @@ Proof.
                 }
             + intros.
               eapply regAssign_renamedApart_agree'; eauto using get_drop, drop_get.
-            + intros. edestruct H8; eauto; dcr. rewrite H20.
-              exploit H2; eauto; dcr. rewrite incl in H27. simpl in *.
-              revert H27; clear_all; cset_tac; intuition.
+            + intros. edestruct H8; eauto; dcr. rewrite H23.
+              exploit H2; eauto; dcr. rewrite incl in H30. simpl in *.
+              revert H30; clear_all; cset_tac; intuition.
               decide (a ∈ of_list (fst Zs)); intuition.
           - eauto with len.
         }
@@ -316,18 +516,20 @@ Require Import Restrict RenamedApart_Liveness LabelsDefined.
     sound for functional liveness and we can thus rely on theorem [regAssign_correct]
     above, which we did prove by induction. *)
 
-Lemma regAssign_correct' s ang ϱ ϱ' (alv:ann (set var)) ZL Lv
+Lemma regAssign_correct' k c (LE:k < c) s ang ϱ ϱ' (alv:ann (set var)) ZL Lv
   : renamedApart s ang
   -> live_sound Imperative ZL Lv s alv
   -> bounded (Some ⊝ Lv \\ ZL) (fst (getAnn ang))
   -> ann_R Subset1 alv ang
   -> noUnreachableCode isCalled s
   -> injective_on (getAnn alv) (findt ϱ 0)
-  -> regAssign s alv ϱ = Success ϱ'
+  -> regAssign c s alv ϱ = Success ϱ'
+  -> sep c (getAnn alv) (findt ϱ 0)
+  -> ann_P (bounded_below c k) alv
   -> locally_inj (findt ϱ' 0) s alv.
 Proof.
   intros.
   eapply renamedApart_live_imperative_is_functional in H0; eauto using bounded_disjoint, renamedApart_disj, meet1_Subset1, live_sound_annotation, renamedApart_annotation.
   eapply regAssign_correct; eauto using locally_inj_subset, meet1_Subset, live_sound_annotation, renamedApart_annotation.
   eapply ann_R_get in H2. destruct (getAnn ang); simpl; cset_tac.
-Qed.u
+Qed.
